Proper word-based vectorization
Basic wordization lemmas

Really complex derivation of wand correctness

src/Assembly/Wordize.v
@@ -1,58 +1,327 @@
 
 Require Export Bedrock.Word Bedrock.Nomega.
-Require Import NArith PArith Ndigits Compare_dec Arith.
-Require Import ProofIrrelevance Ring List.
-Require Export MultiBoundedWord QhasmCommon.
+Require Import NPeano NArith PArith Ndigits Nnat Pnat.
+Require Import Arith Ring List Compare_dec Bool.
+Require Import FunctionalExtensionality.
 
-Import ListNotations.
+Delimit Scope wordize_scope with wordize.
+Local Open Scope wordize_scope.
 
-(* Tuple Manipulations *)
+Notation "& x" := (wordToNat x) (at level 30) : wordize_scope.
 
-Fixpoint Tuple (T: Type) (n: nat): Type :=
-  match n with
-  | O => T
-  | S m => (T * (Tuple T m))%type
-  end.
+Lemma word_size_bound : forall {n} (w: word n),
+  (& w <= pow2 n - 1)%nat.
+Proof. intros; assert (B := wordToNat_bound w); omega. Qed.
 
-Definition just {T} (x: T): Tuple T O := x.
+Lemma pow2_gt0 : forall x, (pow2 x > 0)%nat.
+Proof. intros; induction x; simpl; intuition. Qed.
 
-Definition cross {T n} (x: T) (tup: Tuple T n): Tuple T (S n) := (x, tup).
-
-Definition getLen {T n} (tup: Tuple T n) := (S n).
-
-Fixpoint tget' {T n} (tup: Tuple T n) (x: nat): T.
-  induction x, n; try exact tup.
-
-  exact (fst tup).
-  exact (tget' _ _ (snd tup) x).
-Defined.
-
-Definition tget {T n} (tup: Tuple T n) (x: nat): T :=
-  tget' tup (n - x).
-
-Lemma tget_inc: forall {T k} (x: nat) (v: T) (tup: Tuple T k),
-    (x <= k)%nat -> tget tup x = tget (cross v tup) x.
+Lemma wordize_plus: forall {n} (x y: word n) (b: nat),
+    (&x <= b)%nat
+  -> (&y <= (pow2 n - b - 1))%nat
+  -> (&x + &y) = wordToNat (x ^+ y).
 Proof.
-  intros; unfold cross, tget.
-  replace (S k - x) with (S (k - x)) by intuition.
-  unfold tget'; simpl; intuition.
+  intros; unfold wplus, wordBin;
+    repeat rewrite wordToN_nat in *;
+    repeat rewrite NToWord_nat in *;
+    rewrite <- Nat2N.inj_add; rewrite Nat2N.id.
+
+  destruct (wordToNat_natToWord n (&x + &y)) as [k HW];
+    destruct HW as [HW HK]; rewrite HW; clear HW.
+
+  assert ((&x) + (&y) <= (pow2 n - 1))%nat by (
+    pose proof (word_size_bound x);
+    pose proof (word_size_bound y);
+    omega).
+
+  assert (k * pow2 n <= pow2 n - 1)%nat by omega.
+
+  destruct k; subst; simpl in *; intuition;
+    clear H H0 H1 HK;
+    contradict H2.
+
+  pose proof (pow2_gt0 n).
+  induction k; simpl; intuition.
 Qed.
 
-Ltac tupleize n :=
-  repeat match goal with
-  | [T: Tuple _ ?k, w: word n |- _] => let H := fresh in
-    replace w with (tget (cross w T) (S k)) by (simpl; intuition);
+Lemma wordize_mult: forall {n} (x y: word n) (b: nat),
+    (1 <= n)%nat
+  -> (&x <= b)%nat
+  -> (&y <= (pow2 n - 1) / b)%nat
+  -> (&x * &y)%nat = wordToNat (x ^* y).
+Proof.
+  intros; unfold wmult, wordBin;
+    repeat rewrite wordToN_nat in *;
+    repeat rewrite NToWord_nat in *;
+    rewrite <- Nat2N.inj_mul; rewrite Nat2N.id.
 
-      assert (forall m, (m <= k)%nat -> tget T m = tget (cross w T) m) as H
-        by (intros; apply tget_inc; intuition);
-      repeat rewrite H by intuition;
+  destruct (wordToNat_natToWord n (&x * &y)) as [k HW];
+    destruct HW as [HW HK]; rewrite HW; clear HW.
 
-      generalize (cross w T); clear w T H; intro T
+  assert ((&x) * (&y) <= (pow2 n - 1))%nat. {
+    destruct (Nat.eq_dec b 0); subst;
+      try abstract (replace (&x) with 0 by intuition; omega).
 
-  | [w: word n |- _] =>
-    replace w with (tget (just w) O) by (simpl; intuition);
-      generalize (just w); clear w; let T := fresh in intro T
-  end.
+    transitivity ((&x * (pow2 n - 1)) / b). {
+      transitivity (&x * ((pow2 n - 1) / b)).
 
-(* Conversion from nvec functions to wvec functions *)
+      + apply Nat.mul_le_mono_nonneg_l; intuition.
+      + apply Nat.div_mul_le; assumption.
+    }
 
+    transitivity ((b * (pow2 n - 1)) / (b * 1)). {
+      rewrite Nat.div_mul_cancel_l; intuition.
+      rewrite Nat.div_1_r.
+      apply Nat.div_le_upper_bound; intuition.
+      apply Nat.mul_le_mono_pos_r; intuition.
+      induction n; try inversion H; simpl; intuition.
+      pose proof (pow2_gt0 n).
+      omega.
+    }
+
+    rewrite Nat.div_mul_cancel_l; intuition.
+    rewrite Nat.div_1_r; intuition.
+  }
+
+  assert (k * (pow2 n) <= pow2 n - 1)%nat by omega.
+
+  induction k; try omega.
+
+  assert (pow2 n - 1 < S k * (pow2 n))%nat. {
+    destruct n; try inversion H; simpl; try omega.
+    pose proof (pow2_gt0 n).
+    induction k; try omega.
+    
+    transitivity (pow2 n + pow2 n + pow2 n); try omega.
+    replace (pow2 n + (pow2 n + 0) + S k * _)
+      with (pow2 n + pow2 n + pow2 n +
+           (pow2 n + k * (pow2 n + (pow2 n + 0)))).
+    apply Nat.lt_add_pos_r.
+    apply Nat.add_pos_nonneg; try omega; intuition.
+
+    simpl; omega.
+  }
+
+  contradict H3; omega.
+Qed.
+
+Lemma testbit_pos0: forall p k,
+    testbit (Pos.to_nat p~0) k =
+      match k with | O => false | S k' => testbit (Pos.to_nat p) k' end.
+  intros; destruct k.
+
+  - unfold testbit; simpl; intuition.
+    unfold odd; replace (even _) with true; intuition.
+    symmetry; apply even_spec.
+    exists (Pos.to_nat p).
+    replace (p~0)%positive with (2*p)%positive by intuition.
+    apply Pos2Nat.inj_mul.
+
+  - rewrite (Pos2Nat.inj_xO); intuition.
+    rewrite Nat.testbit_even_succ; intuition.
+Qed.
+
+Lemma testbit_pos1: forall p k,
+    testbit (Pos.to_nat p~1) k =
+      match k with | O => true | S k' => testbit (Pos.to_nat p) k' end.
+  intros; destruct k.
+
+  - unfold testbit; simpl; intuition.
+    apply odd_spec; exists (Pos.to_nat p).
+    replace (p~1)%positive with (2*p + 1)%positive by intuition.
+    rewrite Pos2Nat.inj_add; rewrite Pos2Nat.inj_mul; intuition.
+
+  - rewrite (Pos2Nat.inj_xI); intuition.
+    replace (S (2 * Pos.to_nat p)) with ((2 * Pos.to_nat p) + 1) by intuition.
+    rewrite Nat.testbit_odd_succ; intuition.
+Qed.
+
+Lemma testbit_zero: testbit 0 = (fun (_: nat) => false).
+  apply functional_extensionality; intros;
+      rewrite testbit_0_l; intuition.
+Qed.
+
+Definition even_dec (x: nat): {exists x', x = 2*x'} + {exists x', x = 2*x' + 1}.
+  refine (if (bool_dec (odd x) true) then right _ else left _).
+
+  - apply odd_spec in _H; destruct _H; exists x0. abstract intuition.
+  - unfold odd in _H.
+    assert (even x = true) by abstract (destruct (even x); intuition).
+    apply even_spec in H; destruct H; exists x0; abstract intuition.
+Defined.
+
+Lemma testbit_spec: forall (n x y: nat), (x < pow2 n)%nat -> (y < pow2 n)%nat -> 
+    (forall k, (k < n)%nat -> testbit x k = testbit y k) -> x = y.
+Proof.
+  intro n; induction n; intros. simpl in *; omega.
+  destruct (even_dec x) as [px|px], (even_dec y) as [py|py];
+    destruct px as [x' px], py as [y' py];
+    rewrite px in *; rewrite py in *;
+    clear x y px py;
+    replace (pow2 (S n)) with (2 * (pow2 n)) in * by intuition;
+    assert (x' < pow2 n)%nat by intuition;
+    assert (y' < pow2 n)%nat by intuition.
+
+  - apply Nat.mul_cancel_l; intuition.
+    apply IHn; intuition.
+    assert (S k < S n)%nat as Z by intuition.
+    pose proof (H1 (S k) Z); intuition.
+    repeat rewrite testbit_even_succ in H5; intuition.
+
+  - assert (0 < S n)%nat as Z by intuition.
+    apply (H1 0) in Z.
+    rewrite testbit_even_0 in Z;
+      rewrite testbit_odd_0 in Z;
+      inversion Z.
+
+  - assert (0 < S n)%nat as Z by intuition.
+    apply (H1 0) in Z.
+    rewrite testbit_even_0 in Z;
+      rewrite testbit_odd_0 in Z;
+      inversion Z.
+
+  - apply Nat.add_cancel_r; apply Nat.mul_cancel_l; intuition.
+    apply IHn; intuition.
+    assert (S k < S n)%nat as Z by intuition.
+    pose proof (H1 (S k) Z); intuition.
+    repeat rewrite testbit_odd_succ in H5; intuition.
+Qed. 
+
+Lemma odd_def0: forall x, odd (S (x*2)) = true.
+Proof. intros; intuition. apply odd_spec. exists x. omega. Qed.
+
+Lemma odd_def1: forall x, odd (x * 2) = false.
+Proof.
+  intros; intuition; unfold odd.
+  replace (even _) with true; intuition; symmetry.
+  rewrite even_spec.
+  exists x. omega.
+Qed.
+
+Inductive BinF := | binF: forall (a b c d: bool), BinF.
+
+Definition applyBinF (f: BinF) (x y: bool) :=
+  match f as f' return f = f' -> _ with
+  | binF a b c d => fun _ =>
+    if x
+    then if y
+      then a
+      else b
+    else if y
+      then c
+      else d
+  end eq_refl.
+
+Definition boolToBinF (f: bool -> bool -> bool): {g: BinF | f = applyBinF g}.
+  intros; exists (binF (f true true) (f true false) (f false true) (f false false));
+    abstract (
+      apply functional_extensionality; intro x;
+      apply functional_extensionality; intro y;
+      destruct x, y; unfold applyBinF; simpl; intuition).
+Qed.
+
+Lemma testbit_odd_succ': forall x k, testbit (S (x * 2)) (S k) = testbit x k.
+  intros.
+  replace (S (x * 2)) with ((2 * x) + 1) by omega.
+  apply testbit_odd_succ.
+Qed. 
+
+Lemma testbit_even_succ': forall x k, testbit (x * 2) (S k) = testbit x k.
+  intros; replace (x * 2) with (2 * x) by omega; apply testbit_even_succ.
+Qed. 
+
+Lemma testbit_odd_zero': forall x, testbit (S (x * 2)) 0 = true.
+  intros.
+  replace (S (x * 2)) with ((2 * x) + 1) by omega.
+  apply testbit_odd_0.
+Qed. 
+
+Lemma testbit_even_zero': forall x, testbit (x * 2) 0 = false.
+  intros; replace (x * 2) with (2 * x) by omega; apply testbit_even_0.
+Qed. 
+
+Lemma testbit_bitwp: forall {n} (x y: word n) f k, (k < n)%nat ->
+  testbit (wordToNat (bitwp f x y)) k = f (testbit (&x) k) (testbit (&y) k).
+Proof.
+  intros.
+
+  pose proof (shatter_word x);
+    pose proof (shatter_word y);
+    simpl in *.
+
+  induction n. inversion H. clear IHn; rewrite H0, H1; clear H0 H1; simpl.
+
+  replace f with (applyBinF (proj1_sig (boolToBinF f))) in *
+    by (destruct (boolToBinF f); simpl; intuition);
+    generalize (boolToBinF f) as g; intro g;
+    destruct g as [g pg]; simpl; clear pg f.
+
+  revert x y H; generalize k n; clear k n; induction k, n;
+    intros; try omega. 
+
+  - destruct g as [a b c d], (whd x), (whd y);
+      destruct a, b, c, d; unfold applyBinF in *; clear H;
+      repeat rewrite testbit_odd_zero';
+      repeat rewrite testbit_even_zero';
+      reflexivity.
+
+  - destruct g as [a b c d], (whd x), (whd y);
+      destruct a, b, c, d; unfold applyBinF in *; clear H;
+      repeat rewrite testbit_odd_zero';
+      repeat rewrite testbit_even_zero';
+      reflexivity.
+
+  - assert (k < S n)%nat as HB by omega;
+      pose proof (IHk n (wtl x) (wtl y) HB) as Z; clear HB IHk.
+
+    assert (forall {m} (w: word (S m)),
+      &w = if whd w
+           then S (& wtl w * 2)
+           else & wtl w * 2) as r0. {
+      clear H Z x y; intros.
+      pose proof (shatter_word w); simpl in H; rewrite H; clear H; simpl.
+      destruct (whd w); intuition.
+    } repeat rewrite <- r0 in Z; clear r0.
+
+    assert (forall {m} (a b: word (S m)),
+      & bitwp (applyBinF g) a b
+         = if applyBinF g (whd a) (whd b)
+           then S (& bitwp (applyBinF g) (wtl a) (wtl b) * 2)
+           else & bitwp (applyBinF g) (wtl a) (wtl b) * 2) as r1. {
+      clear H Z x y; intros.
+      pose proof (shatter_word a); pose proof (shatter_word b);
+        simpl in *; rewrite H; rewrite H0; clear H H0; simpl.
+      destruct (applyBinF g (whd a) (whd b)); intuition.
+    } repeat rewrite <- r1 in Z; clear r1.
+
+    destruct g as [a b c d], (whd x), (whd y);
+      destruct a, b, c, d; unfold applyBinF in *; clear H;
+      repeat rewrite testbit_odd_succ';
+      repeat rewrite testbit_even_succ';
+      assumption.
+Qed.
+
+(* (forall k, testbit x k = testbit y k) <-> x = y. *)
+Lemma wordize_and: forall {n} (x y: word n),
+  (Nat.land (&x) (&y))%nat = & (x ^& y).
+Proof.
+  intros n x y.
+  pose proof (pow2_gt0 n).
+  assert (&x < pow2 n)%nat by (pose proof (word_size_bound x); intuition).
+  assert (&y < pow2 n)%nat by (pose proof (word_size_bound y); intuition).
+  apply (testbit_spec n).
+
+  - induction n.
+
+    + simpl in *; intuition.
+      replace (&x) with 0 by intuition.
+      replace (&y) with 0 by intuition.
+      simpl; intuition.
+
+    + admit.
+
+  - pose (word_size_bound (x ^& y)); intuition.
+
+  - intros; rewrite land_spec.
+    unfold wand; rewrite testbit_bitwp; intuition.
+Qed.
